boogie_examples/or.bpl
@@ -1,0 +1,4 @@
+procedure or();
+implementation or(){
+assert 1 == (1 || 3);
+}
