boogie_examples/return.bpl
@@ -1,0 +1,12 @@
+procedure returner() returns(variable: int);
+implementation returner() returns(variable: int) {
+	variable := 1;
+	return;
+}
+procedure test();
+implementation test() {
+var a : int;
+a := 0;
+call a := returner();
+assert a > 0;
+}
